more builtins, better reasoning (see Example.v for an example)

src/BuiltinSem.v
@@ -29,19 +29,66 @@ Definition mb (num_type_args : nat) (num_args : nat) (b : builtin) : Expr :=
   t_e.
 
 
-(* table of builtins, along with their type and val level arity *)
+(* table of builtins, along with their arity *)
 Definition table : list (string * Expr) :=
-  ("demote", mb 2 0 Demote) ::
-  ("+", mb 1 2 Plus) ::
+  ("demote", mb 2 0 Demote) :: (* TESTED *)
+  ("+", mb 1 2 Plus) :: (* TESTED *)
   ("-", mb 1 2 Minus) ::
   ("*", mb 1 2 Times) ::
-  ("/", mb 1 2 Div) ::
+  ("/", mb 1 2 Div) :: 
+  ("%", mb 1 2 Mod) ::
+  ("^^", mb 1 2 Exp) ::
+  ("lg2", mb 1 2 lg2) ::
+  ("True", mb 9 9 true_builtin) ::
+  ("False", mb 9 9 false_builtin) ::
   ("negate", mb 1 1 Neg) ::
+  ("complement", mb 9 9 Compl) ::
+  ("<", mb 1 2 Lt) ::
+  (">", mb 1 2 Gt) ::
+  ("<=", mb 1 2 Le) ::
+  (">=", mb 1 2 Ge) ::
   ("==", mb 1 2 Eq) ::
+  ("!=", mb 1 2 Neq) ::
+  ("&&", mb 1 2 And) ::
+  ("||", mb 1 2 Or) ::
+  ("^", mb 1 2 Xor) ::
+  ("zero", mb 9 9 Zero) ::
+  ("<<", mb 1 2 Shiftl) ::
+  (">>", mb 1 2 Shiftr) ::
+  ("<<<", mb 1 2 Rotl) ::
+  (">>>", mb 1 2 Rotr) ::
+  ("#", mb 1 2 Cons) ::
+  ("splitAt", mb 9 9 splitAt) ::
+  ("join", mb 9 9 join) ::
+  ("split", mb 9 9 split) ::
+  ("reverse", mb 9 9 reverse) ::
+  ("transpose", mb 9 9 transpose) ::
+  ("@", mb 9 9 At) ::
+  ("@@", mb 9 9 AtAt) ::
+  ("!", mb 9 9 Bang) ::
+  ("!!", mb 9 9 BangBang) ::
+  ("update", mb 9 9 update) ::
+  ("updateEnd", mb 9 9 updateEnd) ::
+  ("fromThen", mb 9 9 fromThen) ::
+  ("fromTo", mb 9 9 fromTo) ::
+  ("fromThenTo", mb 9 9 fromThenTo) ::
+  ("infFrom", mb 9 9 infFrom) ::
+  ("infFromThen", mb 9 9 infFromThen) ::
+  ("error", mb 9 9 error) ::
+  ("pmult", mb 9 9 pmult) ::
+  ("pdiv", mb 9 9 pdiv) ::
+  ("pmod", mb 9 9 pmod) ::
+  ("random", mb 9 9 random) ::
+  ("trace", mb 9 9 trace) ::
   nil.
 
 (* Here we have the semantics of all builtins *)
 Inductive eval_builtin : builtin -> list val -> val -> Prop :=
+| eval_demote :
+    forall {ws : nat} {nz : ws <> O} (w n : Z) (b : BitV ws),
+      ws = Z.to_nat w ->
+      b = @repr ws nz n ->
+      eval_builtin Demote ((typ (TCon (TC (TCNum n)) nil)) :: (typ (TCon (TC (TCNum w)) nil)) :: nil) (bits b)
 | eval_plus :
     forall {w : nat} {nz : w <> O} (b1 b2 b3 : BitV w) t,
       b3 = @add w nz b1 b2 ->
@@ -66,7 +113,22 @@ Inductive eval_builtin : builtin -> list val -> val -> Prop :=
 (*     forall {w : nat} {nz : w <> O} (b1 b2 b3 : BitV w) t, *)
 (*       b3 = @exp w nz b1 b2 -> *)
 (*       eval_builtin Exp (t :: (bits b1) :: (bits b2) :: nil) (bits b3) *)
-    
+(* | eval_lg2 : *) (* TODO: what is lg2? log base 2? *)
+(*     forall {w : nat} {nz : w <> O} (b1 b2 b3 : BitV w) t, *)
+(*       b3 = @lg2 w nz b1 b2 -> *)
+(*       eval_builtin lg2 (t :: (bits b1) :: (bits b2) :: nil) (bits b3) *)
+| eval_true :
+    eval_builtin true_builtin nil (bit true)
+| eval_false :
+    eval_builtin false_builtin nil (bit false)
+| eval_negate :
+    forall {w : nat} {nz : w <> O} (b1 b2 : BitV w) t,
+      b2 = @neg w nz b1 ->
+      eval_builtin Neg (t :: (bits b1) :: nil) (bits b2)
+| eval_compl :
+    forall {w : nat} {nz : w <> O} (b1 b2 : BitV w) t,
+      b2 = @not w nz b1 ->
+      eval_builtin Compl (t :: (bits b1) :: nil) (bits b2)
 | eval_eq :
     forall {w : nat} (b1 b2 : BitV w) (b : bool) t,
       b = @eq w b1 b2 ->
@@ -75,11 +137,6 @@ Inductive eval_builtin : builtin -> list val -> val -> Prop :=
     forall {w : nat} {nz : w <> O} (b1 b2 : BitV w) t,
       b2 = @neg w nz b1 ->
       eval_builtin Neg (t :: (bits b1) :: nil) (bits b2)
-| eval_demote :
-    forall {ws : nat} {nz : ws <> O} (w n : Z) (b : BitV ws),
-      ws = Z.to_nat w ->
-      b = @repr ws nz n ->
-      eval_builtin Demote ((typ (TCon (TC (TCNum n)) nil)) :: (typ (TCon (TC (TCNum w)) nil)) :: nil) (bits b)
 .
 
 Fixpoint lookup {A : Type} (s : string) (t : list (string * A)) : option A :=
@@ -94,4 +151,21 @@ Definition find_builtin (s : string) : option Expr :=
 Definition lookup_prim (id : ident) : option Expr :=
   let (_,n) := id in
   find_builtin n.
-              
+
+(* Sanity check to make sure all the prims are in the table above *)
+Lemma id_for_all_prims :
+  forall p,
+  exists s x y,
+    lookup s table = Some (mb x y p).
+Proof.
+  intros. 
+  unfold table.
+  destruct p;
+    unfold lookup;
+    do 3 eexists;
+  match goal with
+  | [ |- context[if string_dec ?X ?Y then _ else _] ] => instantiate (3 := X); simpl; reflexivity
+  end.
+  
+Qed.
+
