verif/Example.v
@@ -35,105 +35,24 @@ Definition id_ge := bind_decl_groups whole_prog gempty.
 
 Definition E := extend empty (12,"input") (bits (@repr width nz 2)).
 
-Ltac e := econstructor; try unfold mb; try reflexivity.
+Ltac ec := econstructor; try unfold mb; try reflexivity.
 Ltac g := eapply eval_global_var; try reflexivity; try (unfold mb; simpl).
 
+Ltac e :=
+  match goal with
+  | [ |- eval_expr _ ?E (EVar ?id) _ ] =>
+    try solve [ec]; g
+  | [ |- _ ] => ec
+  end.
+
 Lemma eval_id :
-  eval_expr id_ge E (EApp (EVar (242,"id")) (EVar (12,"input"))) (bits (@repr width nz 2)).
+    eval_expr id_ge E (EApp (EVar (242,"id")) (EVar (12,"input"))) (bits (@repr width nz 2)).
 Proof.
-  
-  e. unfold id_ge.
-  g.
-  e. e.
-  e.
-  simpl. e.
-  g.
-  e. e.
-  eapply eval_if_f.
-  e. e.
-  e.
-  g.
-  e. 
-
-  e.
-  e.
-  e.
-  e.
-  e. g.
-  e. e.
-  e. repeat e. 
-  e.
-  e. repeat e.
-
-  e. e. e. e.
-  g.
-  e. e. e. e.
-  g.
+  unfold id_ge.
   repeat e.
-  e.
-  e. repeat e.
-  e.
-  e. e. g.
-  e.
-  e. e.
-  e. g.
-
-  e. e. e.
-  e. e. e. g.
-  e. e. e. e. g.
-  e. e. e. repeat e.
-  e. e. repeat e.
-  e. e. repeat e.
-  e.
-
-  eapply eval_if_f.
-  e. e. e. g.
-  e. e. e. e. e. e. g.
-  e. e. e. repeat e.
-  e. e. repeat e.
-  e. e. e. e. g.
-  e. e. e. e. g.
-  e. e. e. repeat e. e.
-  e. e. g.
-  e. e. e. e. g.
-  e. e. e. e. e. e. g.
-  e. e. e. e. g.
-  e. e. e. repeat e. e.
-  e. repeat e. e. e. repeat e. e.
-
-  eapply eval_if_t.
-  e. e. e. g.
-  e. e. e. e. e. e. g.
-  e. e. e. repeat e. e.
-  e. repeat e. e.
-  e. e. g.
-  e. e. e. repeat e.
-  e. e. repeat e. e. e. repeat e.
-  e.
-
+  
   Unshelve.
   all: cbv; omega.
 Qed.
 
-(*
-Definition three_ge := bind_decl_group plus_decl gempty.
-Definition add_1_2 := EApp (EApp (EVar 1) (lit 1)) (lit 2).
 
-Lemma to_three :
-  eval_expr three_ge empty add_1_2 (bits (@repr width nz 3) ).
-Proof.
-  econstructor. unfold three_ge.
-  econstructor.
-  eapply eval_global_var.
-  unfold empty. reflexivity.
-  simpl. reflexivity.
-  econstructor.
-  econstructor.
-  econstructor.
-  econstructor.
-  econstructor.
-  econstructor. unfold extend. simpl. reflexivity.
-  econstructor. unfold extend. simpl. reflexivity.
-  econstructor. exact nz.
-Qed.
-*)
